new/golang/defn/interface.v
@@ -11,14 +11,14 @@ Definition get (f : string) : val :=
   λ: "v",
     let: "v" := (match: "v" with InjL "v" => "v" | InjR <> => #() end) in
     let: (("typeid", "val"), "mset") := "v" in
-    (match: (struct.assocl_lookup #(str f) "mset") with
+    (match: (struct.assocl_lookup #f "mset") with
        InjL <> => #()
      | InjR "m" => "m"
      end) "val"
 .
 
 Local Definition make_def (mset : list (string*val)) : val :=
-  λ: "v", InjL (#(str "NO TYPE IDS YET"), "v", (struct.fields_val mset)).
+  λ: "v", InjL (#"NO TYPE IDS YET", "v", (struct.fields_val mset)).
 Program Definition make := unseal (_:seal (@make_def)). Obligation 1. by eexists. Qed.
 Definition make_unseal : make = _ := seal_eq _.
 
