new/golang/defn/notation.v
@@ -1,6 +1,1 @@
 From Perennial.goose_lang Require Export lang notation.
-
-(*
-#[warnings="-uniform-inheritance"]
-Coercion Var : string >-> expr.
-*)
